\documentclass{article}
\usepackage[usenames]{color}
\usepackage{minted}
\usepackage[utf8]{inputenc}
\usepackage[T1]{fontenc}
\usepackage{graphicx}
\usepackage{grffile}
% Package longtable omitted
% Package wrapfig omitted
% Package rotating omitted
\usepackage[normalem]{ulem}
\usepackage{amsmath}
\usepackage{textcomp}
\usepackage{amssymb}
% Package capt-of omitted
% Package imakeidx omitted
% Package hyperref omitted
\pagestyle{empty}             % do not remove
% The settings below are copied from fullpage.sty
\setlength{\textwidth}{\paperwidth}
\addtolength{\textwidth}{-3cm}
\setlength{\oddsidemargin}{1.5cm}
\addtolength{\oddsidemargin}{-2.54cm}
\setlength{\evensidemargin}{\oddsidemargin}
\setlength{\textheight}{\paperheight}
\addtolength{\textheight}{-\headheight}
\addtolength{\textheight}{-\headsep}
\addtolength{\textheight}{-\footskip}
\addtolength{\textheight}{-3cm}
\setlength{\topmargin}{1.5cm}
\addtolength{\topmargin}{-2.54cm}

\input{preamble.tex}

\begin{document}
$z$
\begin{equation*}
   z=r(\cos\theta+i\sin\theta)
   \end{equation*}
$r=\abs{z}\ge0$
$0\le\theta\le 2\pi$
$z=\cos\theta+i\sin\theta$
$w=\cos\psi+i\sin\psi$
\begin{equation*}
   zw=\cos(\theta+\psi)+i\sin(\theta+\psi)
   \end{equation*}
$\forall x\in\R,n\in\N$
\begin{equation*}
   \cos(nx)+i\sin(nx)=(\cos x+i\sin x)^n
   \end{equation*}
$e^{ix}=\cos x+i\sin x$
$n\in\N\ge 1$
$\xi$
$\xi^n=1$
\begin{equation*}
   e^{2\pi ik/n}=\cos(\frac{2\pi k}{n})+i\sin(\frac{2\pi k}{n})
   \end{equation*}
$k=0,1,\dots,n-1$
\begin{equation*}
   x^n-1=\displaystyle\prod_{\xi^n=1}(x-\xi)
   \end{equation*}
$\xi$
$n$
$\xi$
$d\in\N^+$
\begin{equation*}
   \Phi_d(x)=\displaystyle\prod(x-\xi)
   \end{equation*}
$\xi$
$n\ge 1$
\begin{equation*}
   x^n-1=\displaystyle\prod_{d|n}\Phi_d(x)
   \end{equation*}
\begin{equation*}
   \phi(n)=\deg(\Phi_n(x))
   \end{equation*}
$n\ge1$
$\phi(n)$
$k$
$1\le k\le n$
$(k,n)=1$
$e^{2\pi ik/n}$
$k$
$n$
$n\ge 1$
\begin{equation*}
   n=\displaystyle\sum_{d|n}\phi(d)
   \end{equation*}
$X$
$X$
$X$
$S_X$
$X$
$X=\lb 1,2,\dots,n\rb$
$S_X$
$X_n$
$n$
$i_1,i_2,\dots,i_r$
$\lb 1,2,\dots,n\rb$
$\alpha\in S_n$
\begin{equation*}
   \alpha(i_1)=i_2,\alpha(i_2)=i_3,\dots,\alpha(i_{r-1})=i_r,\alpha(i_r)=i_1
   \end{equation*}
$r$
\begin{equation*}
   \alpha=(i_1\; i_2\;\dots\; i_r)
   \end{equation*}
$\alpha,\beta\in S_n$
$i$
$\alpha,\beta\in S_n$
$\alpha\in S_n$
$k$
$\alpha$
$\alpha$
$\alpha$
$(i)$
$i$
$\alpha$
$\alpha\in S_n$
$\alpha=\beta_1\dots\beta_t$
$i$
$\beta_t(i)\neq i$
$\beta_t^k(i)\neq\beta_t^{k-1}(i)$
$k\ge 1$
$\gamma,\alpha\in S_n$
$\alpha\gamma\alpha^{-1}$
$\gamma$
$\gamma$
\begin{equation*}
   \gamma=\beta_1\beta_2\dots(i_1\; i_2\;\dots)\dots\beta_t
   \end{equation*}
$\alpha\gamma\alpha^{-1}$
$\gamma$
$\alpha$
$\gamma$
\begin{gather*}
   \beta=(1\;2\;3)(4)(5)\\
   \gamma=(5\;2\;4)(1)(3)
   \end{gather*}
$\alpha$
\begin{equation*}
   \alpha=
   \begin{pmatrix}
   1&2&3&4&5\\
   5&2&4&1&3
   \end{pmatrix}
   \end{equation*}
$\gamma$
$\sigma$
$S_n$
$\alpha\in S_n$
$\sigma=\alpha\gamma\alpha^{-1}$
$n\ge 2$
$\alpha\in S_n$
$(1\;2\;\dots\; r)=(1\; r)(1\; r-1)\dots(1\; 2)$
$\alpha\in S_n$
$\alpha\in S_n$
$\alpha=\beta_1\dots\beta_t$
$\alpha$
\begin{equation*}
   \sgn(\alpha)=(-1)^{n-t}
   \end{equation*}
$\alpha,\beta\in S_n$
\begin{equation*}
   \sgn(\alpha\beta)=\sgn(\alpha)\sgn(\beta)
   \end{equation*}
$\alpha\in S_n$
$\sgn(\alpha)=1$
$\alpha$
$\alpha$
$\alpha,\beta\in S_n$
$\alpha$
$\beta$
$\alpha\beta$
$\alpha$
$\beta$
$\alpha\beta$
$G$
\begin{equation*}
   *:G\times G\to G
   \end{equation*}
$G$
$x\in G$
$x'\in G$
$x*x'=e=x'*x$
$G$
$G$
$x*a=x*b$
$a*x=b*x$
$a=b$
$e$
$x\in G$
$(x^{-1})^{-1}=x$
$a_1a_2\dots a_n$
$G$
$a_1,a_2,\dots,a_n\in G$
$a_1a_2\dots a_n$
$G$
$a\in G$
$a^k=1$
$k>1$
$k\ge 1$
$a$
$a$
$G$
$x\in G$
$\varphi:\R^2\to\R^2$
$\Sigma(\pi)$
$\varphi$
$\varphi(\pi)=\pi$
$\Sigma(\pi)$
$\pi_4$
$\Sigma(\pi_4)$
$D_8$
$\pi_n$
$n$
$v_1,\dots,v_n$
$O$
$\Sigma(\pi_n)$
$2n$
$D_{2n}$
$H$
$G$
$1\in H$
$x,y\in H$
$xy\in H$
$x\in H$
$x^{-1}\in H$
$H$
$G$
$H\le G$
$H$
$H$
$G$
$H$
$x,y\in H$
$xy^{-1}\in H$
$H$
$G$
$H$
$a,b\in H$
$ab\in H$
$G$
$a\in G$
\begin{equation*}
   \langle a\rangle=\{a^n:n\in\Z\}=\{\text{all powers of } a\}
   \end{equation*}
$\la a\ra$
$G$
$a$
$G$
$a\in G$
$G=\la a\ra$
$a$
$m$
$\I_m$
$m$
$m\ge 2$
$a\in \Z$
$[a]=[r]$
$r$
$0\le r<m$
$0\le r'<r<m$
$[r']\neq[r]$
$\I_m$
$m$
$G=\la a\ra$
$n$
$a^k$
$G$
$(k,n)=1$
$G$
$n$
$\gen(G)=\{\text{all generators
      of } G\}$
\begin{equation*}
      \abs{\gen(G)}=\phi(n)
      \end{equation*}
$\phi$
$t\in\N$
$a^{kt}=a$
$a^{kt-1}=1$
$n\mid kt-1$
$G$
$a\in G$
$a$
$\abs{\la a\ra}$
$G$
$G$
$\abs{G}$
$G$
$\bigcap_{i\in I}H_i$
$G$
$G$
$X$
$G$
$\la X\ra$
$G$
$X$
$\la X\ra\le H$
$H$
$G$
$X$
$X$
$G$
$\la X\ra$
$X$
$X$
$g\in G$
$g=x_1^{e_1}\dots
   x_n^{e_n}$
$x_i\in X$
$e_i=\pm 1$
$i$
$X$
$G$
$\la X\ra$
$X$
$H\le G$
$a\in G$
$aH$
$aH$
$G$
\begin{equation*}
   aH=\{ah:h\in H\}
   \end{equation*}
$aH$
$Ha$
$H\le G,a,b\in G$
$aH=bH$
$b^{-1}a\in H$
$aH\cap bH\neq\emptyset$
$aH=bH$
$\abs{aH}=\abs{H}$
$a\in G$
$a\equiv b$
$b^{-1}a\in H$
$H$
$G$
$\abs{H}$
$\abs{G}$
$\{a_1H,a_2H,\dots,a_tH\}$
$H$
$G$
\begin{equation*}
   G=a_1H\cup a_2H\cup\dots\cup a_tH
   \end{equation*}
\begin{equation*}
   \abs{G}=\abs{a_1H}+\dots+\abs{a_tH}
   \end{equation*}
$\abs{a_iH}=\abs{H}$
$i$
$\abs{G}=t\abs{H}$
$H$
$G$
$[G:H]$
$H$
$G$
$\abs{G}=[G:H]\abs{H}$
$G$
$a\in G$
$a$
$\abs{G}$
$G$
$a^{\abs{G}}=1$
$a\in G$
$p$
$G$
$p$
$U(\I_m)$
\begin{equation*}
    U(\I_m)=\{[r]\in\I_m:(r,m)=1\}
   \end{equation*}
$\phi(m)$
$p$
$U(\I_m)=\I_m^{\times}$
$\I_p$
$p$
$a\in\Z$
\begin{equation*}
   a^p\equiv a\mod p
   \end{equation*}
$[a^p]=[a]$
$\I_p$
$[a]=[0]$
$[a^p]=[a]^p=[0]$
$\abs{\I_p^\times}=p-1$
$[a]^{p-1}=[1]$
$(r,m)=1$
\begin{equation*}
   r^{\phi(m)}\equiv 1\mod m
   \end{equation*}
$p$
\begin{equation*}
   (p-1)!\equiv -1\mod p
   \end{equation*}
$(G,*)$
$(H,\circ)$
$f:G\to H$
\begin{equation*}
   f(x*y)=f(x)\circ f(y)
   \end{equation*}
$x,y\in G$
$f$
$f$
$G$
$H$
$G\cong H$
$f:G\to H$
$f(1)=1$
$f(x^{-1})=f(x)^{-1}$
$f(x^n)=f(x)^n$
$n\in\Z$
$f:G\to H$
\begin{equation*}
   \tf{kernel}f=\{x\in G:f(x)=1\}
   \end{equation*}
\begin{equation*}
   \tf{image}f=\{h\in H:h=f(x)\text{ for some } x\in G\}
   \end{equation*}
$f:G\to H$
$\ker f$
$G$
$\im f$
$H$
$x\in\ker f$
$a\in G$
$axa^{-1}\in\ker f$
$f$
$\ker f=\{1\}$
$f(a)=f(b)\Leftrightarrow f(ab^{-1})=1$
$K$
$G$
$k\in K$
$g\in G$
$gkg^{-1}\in K$
$K\triangleleft G$
$G$
$a\in G$
$a$
$G$
\begin{equation*}
   gag^{-1}
   \end{equation*}
$g\in G$
$G$
$g\in G$
$\gamma_g:G\to G$
\begin{equation*}
   \gamma_g(a)=gag^{-1}
   \end{equation*}
$a\in G$
$G$
$g\in G$
$\gamma_g:G\to G$
$\gamma_g\circ\gamma_{g^{-1}}=1=\gamma_{g^{-1}}\circ\gamma_g$
$H$
$G$
$g^2\in H$
$g\in G$
$H$
$G$
$H$
$G$
$\bQ$
$GL(2, \C)$
\begin{equation*}
   \bQ=\{I,A,A^2,A^3,B,BA,BA^2,BA^3\}
   \end{equation*}
$I$
\begin{equation*}
   A=
   \begin{pmatrix}
   0&1\\
   -1&0
   \end{pmatrix}, \text{ and }
   B=\begin{pmatrix}
   0&i\\
   i&0
     \end{pmatrix}
   \end{equation*}
$A_4$
$\cals(G)$
$G$
$X,Y\in\cals(G)$
\begin{equation*}
   XY=\{xy:x\in X\text{ and } y\in Y\}
   \end{equation*}
$K\le G$
\begin{equation*}
   gK=Kg
   \end{equation*}
$HK$
$H$
$K$
$G=S_3,H=\la(1\;2)\ra,K=\la(1\;3)\ra$
$H$
$K$
$G$
$HK\le G$
$HK=KH$
$H,K\tril G$
$HK\tril G$
$G/K$
$K$
$G$
$K\tril G$
\begin{equation*}
   aKbK=abK
   \end{equation*}
$a,b\in G$
$G/K$
$aKbK=abKK=abK$
$G/K$
$G$
$K$
$K\tril G$
$\pi:G\to G/K$
$a\mapsto aK$
$f:G\to H$
\begin{equation*}
   \ker f\tril G\quad\text{ and }\quad G/\ker f\cong\im f
   \end{equation*}
$\ker f=K$
$\varphi:G/K\to\im f\le H,aK\mapsto f(a)$
$\varphi$
\begin{tikzcd}
   G \arrow[rr,"f"] \arrow[dr,"\pi"]& &
   H\\ 
   &G/K \arrow[ur,"\varphi"]&
   \end{tikzcd}
$H$
$K$
$G$
\begin{equation*}
   \abs{HK}\abs{H\cap K}=\abs{H}\abs{K}
   \end{equation*}
$f:H\times K\to HK,(h,k)\mapsto hk$
$\abs{f^{-1}(x)}=\abs{H\cap K}$
$x=hk$
\begin{equation*}
   f^{-1}(x)=\{(hd,d^{-1}k):d\in H\cap K\}
   \end{equation*}
$H\tril G, K\le G$
$HK\le G,H\cap K\tril G$
\begin{equation*}
   K/(H\cap K)\cong HK/H
   \end{equation*}
$hkH=kk^{-1}hkH=kh'H=kH$
$H,K\tril G$
$K\le H$
$H/K\tril G/K$
\begin{equation*}
   (G/K)/(H/K)\cong G/H
   \end{equation*}
$K\tril G, \pi:G\to G/K$
\begin{equation*}
   S\mapsto \pi(S)=S/K
   \end{equation*}
$Sub(G;K)$
$S$
$G$
$K$
$Sub(G/K)$
$G/K$
$S/K$
$S^*$
$T\le S\le G$
$T^*\le S^*$
$[S:T]=[S^*:T^*]$
$T\tril S$
$T^*\tril S^*$
$S/T\cong S^*/T^*$
\begin{center}
   \begin{tikzcd}
   G \arrow[d,dash] \arrow[rd]&\\
   S \arrow[d,dash] \arrow[rd] & G/K \arrow[d,dash]\\
   T \arrow[d,dash] \arrow[rd] & S/K=S^* \arrow[d,dash]\\
   K  \arrow[rd] & T/K=T^* \arrow[d,dash]\\
   & \{1\}
   \end{tikzcd}
   \end{center}
$\pi^{-1}\pi=1$
$\pi\pi^{-1}=1$
$[S:T]=[S^*:T^*]$
$sT$
$s^*T^*$
\begin{align*}
   \pi(m)T^*=\pi(n)T^*&\Leftrightarrow \pi(m)\pi(n)^{-1}\in T^*\\
   &\Leftrightarrow mn^{-1}K\in T/K\\
   &\Rightarrow mn^{-1}t^{-1}\in K\\
   &\Rightarrow mn^{-1}=tk\in T\\
   &\Leftrightarrow mT=nT\\
   \end{align*}
$G$
\begin{align*}
   [S^*:T^*]&=\abs{S^*}/\abs{T^*}\\
   &=\abs{S/K}/\abs{T/K}\\
   &=(\abs{S}/\abs{K})/(\abs{T}/\abs{K})\\
   &=\abs{S}/\abs{T}\\
   &=[S:T]
   \end{align*}
$T\tril S$
$T/S\cong (T/K)/(S/K)=T^*/S^*$
$T^*\tril S^*$
\begin{equation*}
   \pi(sts^{-1})\in \pi(s)T^*\pi(s)^{-1}=T^*
   \end{equation*}
$sts^{-1}\in \pi^{-1}(T^*)=T$
$G$
$d$
$\abs{G}$
$G$
$d$
$H$
$K$
$H\times
   K$
$(h,k)$
\begin{equation*}
   (h,k)(h',k')=(hh',kk')
   \end{equation*}
$G$
$G'$
$K\tril G, K'tril G'$
$K\times K'\tril
   G\times G'$
\begin{equation*}
   (G\times G')/(K\times K')\cong (G/K)\times(G'/K')
   \end{equation*}
$G$
$H$
$K$
$H\cap K=\{1\}$
$HK=G$
$G\cong H\times K$
$\abs{HK}\abs{H\cap K}=\abs{H}\abs{K}$
$\varphi:G\to H\times
   K$
$m,n$
\begin{equation*}
   \I_{mn}\cong\I_m\times\I_n
   \end{equation*}
$\Z/\la mn\ra\cong\I_m\times\I_n$
$G$
$a,b\in G$
$m,n$
$(m,n)=1$
$ab$
$mn$
$(m,n)=1$
$\phi(mn)=\phi(m)\phi(n)$
$p$
$\phi(p^e)=p^e-p^{e-1}=p^e(1-\frac{1}{p})$
$n=p_1^{e_1}\dots p_t^{e_t}$
\begin{equation*}
      \phi(n)=n(1-\frac{1}{p_1})\dots(1-\frac{1}{p_t})
      \end{equation*}
$n$
$d$
$d$
$n$
$G$
$x\equiv y$
$\la x\ra=\la
   y\ra$
$x$
$\gen(C)$
$C=\la
   x\ra$
\begin{equation*}
   G=\displaystyle\prod_{C}\gen(C)
   \end{equation*}
$C$
$G$
$\abs{\gen(C)}=\phi(n)$
$G$
$n$
$d$
$n$
$d$
$G$
$n$
$p$
$p$
$n$
$G$
$H\le G, \abs{H}=\abs{K}$
$\abs{H}=[H:K]\abs{K}$
$[H:K]=1$
$H=K$
$\inn(S_3)\cong S_3/Z(S_3)\cong S_3$
$\abs{\aut(S_3)}\le 6$
$\aut(S_3)=\inn(S_3)$
$G$
$S_G$
$\abs{G}=n$
$G$
$S_n$
$a\in G$
$\tau_a(x)=ax$
$x\in G$
$\tau_a$
$\tau_{a^{-1}}$
\begin{equation*}
   \tau_a\tau_{a^{-1}}=\tau_1=\tau_{a^{-1}}\tau_a
   \end{equation*}
$G$
$H\le G$
$n$
$\varphi:G\to S_n$
$\ker\varphi\le H$
$H=\{1\}$
$G$
$\I_4$
$\bV$
$\I_4\not\cong\bV$
$G$
$G$
$x,y\neq 1$
$xy\neq x,y$
$G=\{1,x,y,xy\}$
$G$
$G$
$\I_6$
$S_3$
$\I_6\not\cong S_3$
$G$
$\abs{G}$
$t$
$G$
$a$
$H=\{1,a,t,at\}$
$b$
$bt$
$G$
$G$
$G$
$G$
$s$
$\abs{\la s\ra}=3$
$[G:\la s\ra]=\abs{G}/\abs{\la s\ra}=2$
$\la
   s\ra$
$t=t^{-1}$
$tst\in\la s\ra$
$tst=s^0=1$
$s=1$
$tst=s$
$\abs{\la st\ra}=6$
$tst=s^2=s^{-1}$
$H=\la t\ra$
$\varphi:G\to S_{G/\la t\ra}$
\begin{equation*}
   \varphi(g):x\la t\ra\to gx\la t\ra
   \end{equation*}
$\ker\varphi\le\la t\ra$
$\ker\varphi=\{1\}$
$\ker\varphi=\la t\ra$
\end{document}
%%Local Variables:
%%TeX-master: t
%%End:
